runtime/coq/ExtractPositiveSerializerDeps.v
@@ -2,3 +2,4 @@ Require Export Cheerios.BasicSerializers.
 Require Export Cheerios.Core.
 Require Export Cheerios.Types.
 Require Export Cheerios.ExtrCheerios.
+Require Export Cheerios.ExtrIOStream.
