runtime/coq/ExtractTreeSerializer.v
@@ -1,25 +1,28 @@
 Require Import Cheerios.ExtractTreeSerializerDeps.
 Require Import Cheerios.BasicSerializers.
+Require Import Cheerios.IOStream.
 
 Require Import ZArith.
 Require Import ExtrOcamlBasic.
 Require Import ExtrOcamlString.
 
-Import ByteListSerializer.
+Module ByteListBasics := BasicSerializers ByteListWriter ByteListReader.
+Module IOStreamBasics := BasicSerializers IOStream ByteListReader.
+Module ByteListTree := TreeSerializer ByteListWriter ByteListReader.
+Module IOStreamTree := TreeSerializer IOStream ByteListReader.
 
-Check serialize_top.
-Check serialize.
+Locate serialize.
+Check ByteListTree.RWCombinators.RWBasic.bool_Serializer.
+Definition tree_serialize_bytelist_top :=
+  ByteListBasics.RWClass.serialize_top (tree bool)
+                                       (ByteListTree.tree_Serializer ByteListBasics.bool_Serializer). 
 
-Definition tree_serialize_top : tree bool -> Serializer.wire :=
-  serialize_top _ serialize.
-
-Definition tree_deserialize_top : Serializer.wire -> option (tree bool) :=
+Check tree_serialize_bytelist_top.
+Definition tree_deserialize_bytelist_top : ByteListWriter.wire -> option (tree bool) :=
   deserialize_top _ deserialize.
-
-Definition tree_serialize_top' (t : tree bool) : Serializer.wire :=
-  Serializer.wire_wrap (tree_serialize' _ t).
 
 Extraction "runtime/ocaml/tree_serializer.ml"
            map tree_map'
            tree_serialize_top'
            tree_serialize_top tree_deserialize_top.
+*)
